src/algebraic/AG_algebra_theory.v
@@ -1,0 +1,171 @@
+Require Import Setoid Morphisms.
+Require Import Ensembles.
+
+Require Import List.
+Import ListNotations.
+Require Import Sorting.Permutation.
+
+Require Import GraphVerification.src.util.NatSet.
+
+Require Import GraphVerification.src.RG.
+Require Import GraphVerification.src.RG_theory.
+
+Require Import GraphVerification.src.algebraic.AG.
+Require Import GraphVerification.src.algebraic.AG_to_RG.
+
+(** Stating and proving Lemmas and THeorems about the algebraic properties of AGs 
+    A noteworthy result is that we show that
+    the definition-based interpretation of an AG is equivalent to the algebraic interpretation *)
+
+
+(** This is used to verify that the axioms on the algebra of AGs are consistent
+    with the interpretation of the expressions in terms of RGs *)
+Ltac AG_axiom_proof_automation_via_RG :=
+    unfold AG_equiv; simpl; firstorder.
+
+(* These are the "8 axioms" as presented in "Algebraic graphs with class (functional pearl)" by Mokhov *)
+
+(* +++ is commutative and associative *)
+Theorem AG_overlay_Commutative {A : Type} : forall (ag1 ag2 : AG A), ag1 +++ ag2 ==A ag2 +++ ag1.
+Proof.
+    AG_axiom_proof_automation_via_RG.
+Qed.
+
+Theorem AG_overlay_Associative {A : Type} : forall (ag1 ag2 ag3 : AG A), ag1 +++ (ag2 +++ ag3) ==A (ag1 +++ ag2) +++ ag3.
+Proof.
+    AG_axiom_proof_automation_via_RG.
+Qed.
+
+(* (G, ***, e) is a monoid *)
+Theorem AG_empty_connect_L_Identity {A : Type} : forall (ag : AG A),
+    AG_empty *** ag ==A ag.
+Proof.
+    AG_axiom_proof_automation_via_RG.
+Qed.
+
+Theorem AG_empty_connect_R_Identity {A : Type} : forall (ag : AG A),
+    ag *** AG_empty ==A ag.
+Proof.
+    AG_axiom_proof_automation_via_RG.
+Qed.
+
+Theorem AG_connect_Associative {A : Type} : forall (ag1 ag2 ag3 : AG A),
+    ag1 *** (ag2 *** ag3) ==A (ag1 *** ag2) *** ag3.
+Proof.
+    AG_axiom_proof_automation_via_RG.
+Qed.
+
+(* *** distributes over +++ *)
+Theorem AG_connect_overlay_L_Distributes {A : Type} : forall (ag1 ag2 ag3 : AG A),
+    ag1 *** (ag2 +++ ag3) ==A ag1 *** ag2 +++ ag1 *** ag3.
+Proof.
+    AG_axiom_proof_automation_via_RG.
+Qed.
+
+Theorem AG_connect_overlay_R_Distributes {A : Type} : forall (ag1 ag2 ag3 : AG A),
+    (ag1 +++ ag2) *** ag3 ==A ag1 *** ag3 +++ ag2 *** ag3.
+Proof.
+    AG_axiom_proof_automation_via_RG.
+Qed.
+
+(* Decomposition *)
+Theorem AG_connect_Decomposition {A : Type} : forall (ag1 ag2 ag3 : AG A),
+    ag1 *** ag2 *** ag3 ==A ag1 *** ag2 +++ ag1 *** ag3 +++ ag2 *** ag3.
+Proof.
+    AG_axiom_proof_automation_via_RG.
+Qed.
+
+
+
+
+(** Section to make rewrite work with ==A of overlays and connects *)
+
+(* This proof is based on ==R being an equivalence relation *)
+Instance AG_Equivalence {A : Type} : Equivalence (@AG_equiv A).
+Proof.
+    G_derived_equivalence_prover A unit (@AG_to_RG A).
+Qed.
+
+Ltac Proper_proof_automation := split; simpl in *; firstorder.
+
+Instance Proper_overlay {A : Type} : Proper ((@AG_equiv A) ==> AG_equiv ==> AG_equiv) AG_overlay.
+Proof.
+    Proper_proof_automation.
+Qed.
+
+Instance Proper_connect {A : Type} : Proper ((@AG_equiv A) ==> AG_equiv ==> AG_equiv) AG_connect.
+Proof.
+    Proper_proof_automation.
+Qed.
+
+
+
+(** The following theorems are provable using the same automation as the 8 axioms,
+    but this section aims to demonstrate their utility, by using only them.
+    This has already been done in the Agda formalization by Andrey Mokhov *)
+
+(* This is a helper for multiple theorems *)
+Lemma _overlay_preidempotence {A : Type}: forall (ag : AG A), ag +++ ag +++ AG_empty ==A ag.
+Proof.
+    intros.
+    pose proof (AG_connect_Decomposition ag AG_empty AG_empty).
+
+    rewrite AG_empty_connect_R_Identity in H.
+    rewrite AG_empty_connect_R_Identity in H.
+    rewrite <- H.
+
+    reflexivity.
+Qed.
+
+
+(* Identity of + *)
+Theorem AG_empty_overlay_R_Identity {A : Type}: forall (g : AG A), g +++ AG_empty ==A g.
+Proof.
+    intros.
+    rewrite <- _overlay_preidempotence.
+
+    rewrite <- AG_overlay_Associative.
+    rewrite (AG_overlay_Associative AG_empty (g +++ AG_empty)). 
+    rewrite (AG_overlay_Commutative AG_empty (g +++ AG_empty)).
+    rewrite <- AG_overlay_Associative.
+    rewrite <- AG_overlay_Associative.
+
+    rewrite _overlay_preidempotence.
+    rewrite _overlay_preidempotence.
+    reflexivity.
+Qed.
+
+
+(* Idempotence of + *)
+Theorem AG_overlay_Idempotence {A : Type}: forall (ag : AG A), ag +++ ag ==A ag.
+Proof.
+    intros.
+    pose proof _overlay_preidempotence ag.
+    rewrite AG_empty_overlay_R_Identity in H.
+    assumption.
+Qed.
+
+
+(* Absorption *)
+Theorem AG_Absorption {A : Type}: forall (ag1 ag2 : AG A), ag1 *** ag2 +++ ag1 +++ ag2 ==A ag1 *** ag2.
+Proof.
+    intros. pose proof AG_connect_Decomposition ag1 ag2 AG_empty.
+    rewrite (AG_connect_Associative) in H.
+    rewrite AG_empty_connect_R_Identity in H.
+    rewrite AG_empty_connect_R_Identity in H.
+    rewrite AG_empty_connect_R_Identity in H.
+    symmetry in H.
+    assumption.
+Qed.
+
+
+(* Saturation *)
+Theorem AG_Saturation {A : Type}: forall (ag : AG A), ag *** ag *** ag ==A ag *** ag.
+Proof.
+    intros.
+    rewrite AG_connect_Decomposition.
+
+    rewrite AG_overlay_Idempotence.
+    rewrite AG_overlay_Idempotence.
+    reflexivity.
+Qed.
