src/inductive/IG_to_RG.v
@@ -8,8 +8,7 @@ Require Import GraphVerification.src.inductive.IG.
 Require Import GraphVerification.src.inductive.IG_wf_algorithms.
 
 
-(* Defining how an IG converts to an RG *)
-
+(** Defining how an IG converts to an RG *)
 
 Definition RG_and {A B : Type} (c : Context A B) (rg : RG_unlE nat) : RG_unlE nat.
 Proof.
@@ -17,7 +16,8 @@ Proof.
     refine {|
         RG_nodes := fun (n : nat) => (Ensemble_add node rg.(RG_nodes)) n;
         RG_edges := fun (n1 n2 : nat) l => rg.(RG_edges) n1 n2 l \/
-                                            (not (rg.(RG_nodes) node) /\ (Ensemble_add node rg.(RG_nodes)) n1 /\ (Ensemble_add node rg.(RG_nodes)) n2 /\
+                                            (not (rg.(RG_nodes) node)
+                                                /\ (Ensemble_add node rg.(RG_nodes)) n1 /\ (Ensemble_add node rg.(RG_nodes)) n2 /\
                                                 ((In n1 (map snd froms) /\ n2 = node)
                                                     \/ (n1 = node /\ In n2 (map snd tos))
                                                 )
@@ -29,12 +29,15 @@ Defined.
 
 Notation "c &R ig" := (RG_and c ig) (at level 59, right associativity).
 
-
+(* At the moment, this conversion is a little imperfect with respect to edges:
+    In case of adding invalid contexts to the graph, for IGs, invalid neighbors may make it in,
+    wheras for RGs, they are not allowed to be in *)
 Definition IG_to_RG {A B : Type} (ig : IG A B) : RG_unlE nat :=
     IG_ufold RG_and RG_empty ig.
 
 
-(* This ignores labels for now *)
+(* Two IGs are equivalent, if their RGs are equivalent.
+    For now, labels are not taken into account *)
 Definition IG_equiv {A B : Type} (ig1 ig2 : IG A B) : Prop :=
     RG_equiv (IG_to_RG ig1) (IG_to_RG ig2).
 
