src/util/NatSet.v
@@ -1,6 +1,8 @@
 Require Import MSets.
 
-(* Instantiate an FSet module, such that it is the same across the whole project *)
+(** Instantiate an FSet module, such that it is the same across the whole project
+    Also proves some generally useful lemmas about MSets *)
+
 
 Definition Node := Nat_as_OT.t.
 
@@ -11,3 +13,22 @@ Module SProps := EqProperties(NatSet).
 (* Custom additional function for NatSets "fromList" *)
 Definition NatSet_fromList (l : list Node) : NatSet.t :=
     fold_right NatSet.add NatSet.empty l.
+
+
+
+
+Lemma NatSet_In_is_In_elements : forall (x : Node) (s : NatSet.t),
+    NatSet.In x s <-> In x (NatSet.elements s).
+Proof.
+    intros. rewrite <- NatSet.elements_spec1. rewrite SetoidList.InA_alt. firstorder. subst. auto.
+Qed.
+
+Lemma NatSet_NoDup_elements : forall (s : NatSet.t),
+    NoDup (NatSet.elements s).
+Proof.
+    intros. pose proof (NatSet.elements_spec2w s). induction (NatSet.elements s).
+    - apply NoDup_nil.
+    - inversion H. apply NoDup_cons.
+        + unfold not in *. intros. apply H2. apply SetoidList.InA_alt. exists a. auto.
+        + apply IHl. assumption.
+Qed.
